set up parametric simd interface

src/SIMD_ops.ml
@@ -1,0 +1,8 @@
+let app_vunop_str op v =
+  v
+
+let app_vbinop_str op v1 v2 = 
+  v1
+
+let app_vternop_str op v1 v2 v3 =
+  v1
