src/SIMD_ops.mli
@@ -1,0 +1,5 @@
+val app_vunop_str : Big_int_Z.big_int -> char list -> char list
+
+val app_vbinop_str : Big_int_Z.big_int * (Big_int_Z.big_int list) -> char list -> char list -> char list
+
+val app_vternop_str : Big_int_Z.big_int -> char list -> char list -> char list -> char list
