src/convert.ml
@@ -3,35 +3,14 @@ let rec to_nat = function
   | n when n > 0 -> Extract.S (to_nat (n - 1))
   | _ -> failwith "not a nat"
 
-let rec to_positive z =
-  if z < 1 then failwith "not a positive"
-  else if z = 1 then Extract.XH
-  else 
-    let pos' = to_positive (z / 2) in
-    let d = z mod 2 in
-    if d = 0 then
-      Extract.XO pos'
-    else 
-      Extract.XI pos'
-
-let to_n z =
-  if z = 0 then Extract.N0
-  else Npos (to_positive z)
-
 let rec from_nat = function
   | Extract.O -> 0
   | Extract.S n -> 1 + from_nat n
 
-let rec from_positive = function
-  | Extract.XH -> 1
-  | Extract.XO p -> 2 * from_positive p
-  | Extract.XI p -> 1 + 2 * from_positive p
+let z_of_int x =
+  Big_int_Z.big_int_of_int x
 
-let from_z = function
-  | Extract.Z0 -> 0
-  | Extract.Zpos p -> from_positive p
-  | Extract.Zneg p -> - from_positive p
-
-let from_n = function
-  | Extract.N0 -> 0
-  | Extract.Npos p -> from_positive p
+let int_of_z z =
+  if Big_int_Z.is_int_big_int z then 
+    Big_int_Z.int_of_big_int z
+else invalid_arg "int_of_z overflow"
