src/convert.mli
@@ -1,22 +1,9 @@
 (** Convert [int] to [Extract.nat]. **)
 val to_nat : int -> Extract.nat
 
-(** Convert [int] to [Extract.positive]. **)
-val to_positive : int -> Extract.positive
-
-(** Convert [int] to [Extract.n]. **)
-val to_n : int -> Extract.n
-
 (** Convert [Extract.nat] to [int]. **)
 val from_nat : Extract.nat -> int
 
-(** Convert [Extract.positive] to [int]. *)
-val from_positive : Extract.positive -> int
+val z_of_int: int -> Big_int_Z.big_int
 
-(** Convert [Extract.z] to [int]. *)
-val from_z : Extract.z -> int
-
-(** Convert [Extract.n] to [int]. *)
-val from_n : Extract.n -> int
-
-
+val int_of_z: Big_int_Z.big_int -> int
