theories/simd.v
@@ -1,5 +1,5 @@
 From mathcomp Require Import ssreflect ssrbool eqtype seq ssrnat.
-From Coq Require Import BinInt BinNat NArith Lia Uint63.
+From Coq Require Import BinInt BinNat NArith Lia Uint63 String.
 From Wasm Require Import numerics bytes memory common.
 
 Set Implicit Arguments.
@@ -12,6 +12,9 @@ Module Type SIMD_Type.
 
   Parameter v128_default: v128.
 
+  Parameter encode_v128 : v128 -> string.
+  Parameter decode_v128 : string -> v128.
+
 End SIMD_Type.
 
 Module SIMD <: SIMD_Type.
@@ -19,5 +22,39 @@ Module SIMD <: SIMD_Type.
   Definition v128 := bytes.
 
   Definition v128_default : v128 := nil.
-  
+
+Definition encode_v128 bs :=
+  let coq_bytes :=
+    List.map byte_of_compcert_byte bs in
+  string_of_list_byte coq_bytes.
+
+Definition decode_v128 s :=
+  let bs := list_byte_of_string s in
+    List.map compcert_byte_of_byte bs.
+
+Lemma decode_encode_v128: forall v,
+    decode_v128 (encode_v128 v) = v.
+Proof.
+  induction v => //=.
+  unfold decode_v128, encode_v128 in *.
+  rewrite list_byte_of_string_of_list_byte => /=.
+  rewrite list_byte_of_string_of_list_byte in IHv => /=.
+  rewrite IHv.
+  f_equal.
+  by rewrite compcert_byte_roundtrip.
+Qed.
+
+Lemma encode_decode_v128: forall s,
+    encode_v128 (decode_v128 s) = s.
+Proof.
+  induction s => //=.
+  unfold decode_v128, encode_v128 in * => /=.
+  rewrite coq_byte_roundtrip => /=.
+  cbn; f_equal.
+  - by rewrite Ascii.ascii_of_byte_of_ascii.
+  - by apply IHs. 
+Qed.
+
 End SIMD.
+
+Module Export simd_export := SIMD.
